lib/Benchmarks/EdgeTransProof.v
@@ -4,18 +4,12 @@ Declare ML Module "mirrorsolve".
 
 SetSMTSolver "cvc4".
 
-Lemma ethernet_equiv:
+Lemma edge_equiv:
   lang_equiv_state
     (P4A.interp Plain.aut)
     (P4A.interp Optimized.aut)
     Plain.ParseEth0
     Optimized.State_0.
-Proof.
-  eapply lang_equiv_to_pre_bisim.
-  time "init prebisim" intros;
-  unfold mk_init;
-  erewrite Reachability.reachable_states_wit_conv.
-  2: repeat time "constructor" econstructor.
-  2: unfold Reachability.reachable_states_wit;
-     solve_fp_wit.
-Time Admitted.
+Proof. 
+  time "edge lang equiv" solve_lang_equiv_state_axiom Plain.state_eqdec Optimized.state_eqdec true.
+Time Qed.
