lib/Benchmarks/EthernetProof.v
@@ -12,14 +12,5 @@ Lemma ethernet_equiv:
     Reference.SPref
     Combined.Parse.
 Proof.
-  eapply lang_equiv_to_pre_bisim;
-  time "init prebisim" (intros;
-  unfold mk_init;
-  erewrite Reachability.reachable_states_wit_conv; [
-    | repeat econstructor
-    | unfold Reachability.reachable_states_wit;
-      solve_fp_wit
-  ]; simpl).
-Admitted.
-  (* solve_lang_equiv_state_axiom Reference.state_eqdec Combined.state_eqdec false.
-Time Qed. *)
+  solve_lang_equiv_state_axiom Reference.state_eqdec Combined.state_eqdec false.
+Qed.
