lib/NtupleProofs.v
@@ -509,3 +509,18 @@ Proof.
   subst.
   reflexivity.
 Qed. *)
+
+Lemma concat_emp' :
+  forall n (t: n_tuple bool n), 
+    n_tup_wf t ->
+    n_tuple_concat n_tuple_emp t = t.
+Proof.
+  intros.
+  inversion H.
+  apply JMeq_eq.
+  compute.
+  destruct t.
+  simpl in *.
+  erewrite H1.
+  reflexivity.
+Qed.
